BasicSerializers.v
@@ -312,11 +312,13 @@ Proof.
   now rewrite Nnat.Nat2N.id.
 Qed.
 
-Instance nat_Serializer : Serializer nat :=
-  {| serialize := nat_serialize;
-     deserialize := nat_deserialize;
-     serialize_deserialize_id := nat_serialize_deserialize_id
-  |}.
+Instance nat_Serializer : Serializer nat.
+Proof.
+  exact {| serialize := nat_serialize;
+           deserialize := nat_deserialize;
+           serialize_deserialize_id := nat_serialize_deserialize_id
+        |}.
+Qed.
 
 (* Serializer for the standard library's Fin.t based on converting to nat. *)
 Definition Fin_serialize {n} (x : Fin.t n) : Serializer.t :=
